pancake/semantics/timePropsScript.sml
@@ -1,0 +1,80 @@
+(*
+  semantics for timeLang
+*)
+
+open preamble
+     timeLangTheory timeSemTheory
+     pan_commonPropsTheory
+
+val _ = new_theory "timeProps";
+
+val _ = set_grammar_ancestry
+        ["timeLang","timeSem",
+         "pan_commonProps"];
+
+
+Theorem fdom_reset_clks_eq_clks:
+  ∀fm clks.
+    EVERY (λck. ck IN FDOM fm) clks ⇒
+    FDOM (resetClocks fm clks) = FDOM fm
+Proof
+  rw [] >>
+  fs [resetClocks_def] >>
+  fs [FDOM_FUPDATE_LIST] >>
+  ‘LENGTH clks = LENGTH (MAP (λx. 0:num) clks)’ by fs [] >>
+  drule MAP_ZIP >>
+  fs [] >>
+  strip_tac >> pop_assum kall_tac >>
+  ‘set clks ⊆ FDOM fm’ by (
+    fs [SUBSET_DEF] >>
+    rw [] >>
+    fs [EVERY_MEM]) >>
+  fs [SUBSET_UNION_ABSORPTION] >>
+  fs [UNION_COMM]
+QED
+
+
+Theorem reset_clks_mem_flookup_zero:
+  ∀clks ck fm.
+    MEM ck clks ⇒
+    FLOOKUP (resetClocks fm clks) ck = SOME 0
+Proof
+  rw [] >>
+  fs [timeSemTheory.resetClocks_def] >>
+  fs [MEM_EL] >> rveq >>
+  match_mp_tac update_eq_zip_map_flookup >> fs []
+QED
+
+
+
+Theorem reset_clks_not_mem_flookup_same:
+  ∀clks ck fm v.
+    FLOOKUP fm ck = SOME v ∧
+    ~MEM ck clks ⇒
+    FLOOKUP (resetClocks fm clks) ck = SOME v
+Proof
+  rw [] >>
+  fs [timeSemTheory.resetClocks_def] >>
+  last_x_assum (mp_tac o GSYM) >>
+  fs [] >>
+  strip_tac >>
+  match_mp_tac flookup_fupdate_zip_not_mem >>
+  fs []
+QED
+
+
+Theorem flookup_reset_clks_leq:
+  ∀fm ck v tclks q.
+    FLOOKUP fm ck = SOME v ∧ v ≤ q ⇒
+    ∃v. FLOOKUP (resetClocks fm tclks) ck = SOME v ∧ v ≤ q
+Proof
+  rw [] >>
+  cases_on ‘MEM ck tclks’
+  >- (
+    drule reset_clks_mem_flookup_zero >>
+    fs []) >>
+  drule reset_clks_not_mem_flookup_same >>
+  fs []
+QED
+
+val _ = export_theory();
